[Case study] More theory about SCP

Examples/DSL/SCPTheory.lean
@@ -1,131 +1,267 @@
 import Aesop
 import Mathlib.Data.Set.Basic
 
--- CHECK come from the "longer" file
-class PersonalQuorums {Node : Type u} (quorum_of : Node → Set Node → Prop) where
-  quorum_assm : ∀ p p' Q, quorum_of p Q → p' ∈ Q → quorum_of p' Q
+-- adapted from [FBA.thy](https://github.com/stellar/scp-proofs/blob/ac41c6353fae870c47c0e7ee558da98c03a7d041/FBA.thy)
 
--- CHECK come from the "longer" file
-namespace PersonalQuorums
+/-
+  NOTE: For now we do not prove liveness property in Veil, so we only
+  adapt the definitions that are sufficient for justifying the assumptions
+  in the current Veil model of SCP.
+-/
 
-variable {Node : Type u} (quorum_of : Node → Set Node → Prop)
-open PersonalQuorums
+theorem Set.ne_empty_iff_exists_mem {α : Type u} {s : Set α} : s ≠ ∅ ↔ ∃ a, a ∈ s := by
+  rw [← Set.nonempty_iff_ne_empty] ; aesop
 
-def quorum_of_set (S Q : Set Node) : Prop := ∃ p ∈ S, quorum_of p Q
-
--- NOTE: this definition is the same as the one in the DISC'19 paper,
--- but different from the one in the FMBC'20 paper!
--- in the FMBC'20 paper, the conclusion should be like `S ∩ Q ∩ Q' ≠ ∅`
-def is_intertwined (W S : Set Node) : Prop :=
-  S ⊆ W ∧ (∀ Q Q', quorum_of_set quorum_of S Q → quorum_of_set quorum_of S Q' → W ∩ Q ∩ Q' ≠ ∅)
-
--- simply by definition
-lemma qi_intertwined (W S Q1 Q2 : Set Node) (n1 n2 : Node) :
-  is_intertwined quorum_of W S → n1 ∈ S → n2 ∈ S →
-  quorum_of n1 Q1 → quorum_of n2 Q2 →
-  ∃ n3, n3 ∈ W ∧ n3 ∈ Q1 ∧ n3 ∈ Q2 := by
-  unfold is_intertwined quorum_of_set
-  simp only [forall_exists_index, and_imp]
-  intro h1 h2 h3 h4 h5 h6
-  specialize h2 _ _ _ h3 h5 _ h4 h6
-  rewrite [← Set.nonempty_iff_ne_empty] at h2
-  cases h2 ; aesop
-
-end PersonalQuorums
-
-namespace StellarQuorums
+namespace FBA
 
 def project {α β : Type} (slices : β → Set (Set α)) (S : Set α) : β → Set (Set α) :=
   fun n => { Sl ∩ S | Sl ∈ slices n }
 
--- FIXME: might be better to lift `Node` as an argument?
 class System where
   Node : Type
   /-- The set of well-behaved nodes. -/
   W : Set Node
   slices : Node → Set (Set Node)
+  /-- The set of slices of a well-behaved node is not empty. -/
   slices_ne : ∀ p ∈ W, slices p ≠ ∅
 
-def project_system (s : System) (I : Set s.Node) : System :=
-  { Node := s.Node
-    W := s.W
-    slices := project s.slices I
+/-- Restrict all slices in `sys` to only include nodes from `I`.
+    See how it is used in the definition of `intertwined`. -/
+def System.project (sys : System) (I : Set sys.Node) : System :=
+  { Node := sys.Node
+    W := sys.W
+    slices := FBA.project sys.slices I
     slices_ne := by
-      unfold project
-      have h := s.slices_ne
-      intro p hin ; specialize h _ hin
-      rewrite [← Set.nonempty_iff_ne_empty] at h ⊢
-      rcases h with ⟨Sl, h⟩ ; constructor ; aesop }
+      intro p hin
+      unfold FBA.project
+      have h := sys.slices_ne _ hin
+      rw [Set.ne_empty_iff_exists_mem] at h ⊢ ; aesop }
 
 variable [inst : System]
 open System
 
+/-- A quorum is a set whose well-behaved members have at least one slice
+    included in the set. -/
 def quorum (Q : Set Node) : Prop := ∀ p ∈ Q ∩ W, ∃ Sl ∈ slices p, Sl ⊆ Q
 
-lemma quorum_after_proj (Q I : Set Node) : quorum (inst := inst) Q → quorum (inst := project_system inst I) Q := by
-  rcases inst with ⟨Node, W, slices, slices_ne⟩
-  unfold quorum project_system project ; simp
-  intro hq p h1 h2 ; specialize hq _ h1 h2 ; rcases hq with ⟨Sl, hq1, hq2⟩
-  exists Sl ; apply And.intro ; assumption
-  rw [Set.subset_def] at hq2 ⊢ ; simp ; aesop     -- well, just by def
+/-- A set `S` is a slice-blocking set for a node `p` when every slice of
+    `p` intersects `S`. -/
+def blocks_slices (S : Set Node) (p : Node) : Prop :=
+  ∀ Sl ∈ slices p, Sl ∩ S ≠ ∅
+
+/-- A set of node is intertwined if all of its members are well-behaved
+    and it satisfies the quorum intersection property. -/
+structure intertwined (S : Set Node) where
+  well_behaved : S ⊆ W
+  /-- The quorum intersection property; `project`ing the system to `S`
+      allows for the worst-case quorums that might arise.
+      Check [the original FMBC'20 paper](https://drops.dagstuhl.de/storage/01oasics/oasics-vol084-fmbc2020/OASIcs.FMBC.2020.9/OASIcs.FMBC.2020.9.pdf) and
+      [the DISC'19 paper](https://drops.dagstuhl.de/storage/00lipics/lipics-vol146-disc2019/LIPIcs.DISC.2019.27/LIPIcs.DISC.2019.27.pdf)
+      for more information. -/
+  q_inter : (∀ Q Q',
+    quorum (inst := inst.project S) Q →
+    quorum (inst := inst.project S) Q' →
+    Q ∩ S ≠ ∅ → Q' ∩ S ≠ ∅ → Q ∩ Q' ∩ S ≠ ∅)
+
+/-- A set of node is intact if all of its members are well-behaved
+    and it satisfies both the quorum availability property and
+    the quorum intersection property. -/
+structure intact (I : Set Node) extends intertwined I where
+  /-- The quorum availability property: `I` itself is a quorum. -/
+  q_avail : quorum (inst := inst) I
+
+theorem intact_implies_intertwined : ∀ I, intact I → intertwined I := by
+  intro I h ; cases h ; assumption
+
+theorem intertwined_node_is_well_behaved : ∀ n S, intertwined S → n ∈ S → n ∈ W := by
+  intro n S ⟨h, _⟩ ; aesop
+
+theorem intact_node_is_well_behaved : ∀ n I, intact I → n ∈ I → n ∈ W := by
+  intro n S h ; apply intertwined_node_is_well_behaved ; apply intact_implies_intertwined _ h
+
+theorem slice_blocks_ne : ∀ n S I, intact I → n ∈ I → blocks_slices S n →
+    S ∩ I ≠ ∅ := by
+  intro n S I hI hin hblock
+  unfold blocks_slices at hblock
+  have h := hI.q_avail ; unfold quorum at h
+  simp at h ; specialize h _ hin (intact_node_is_well_behaved _ _ hI hin)
+  rcases h with ⟨Sl, hSl, h⟩ ; specialize hblock _ hSl
+  rw [Set.ne_empty_iff_exists_mem] at hblock ⊢ ; simp at hblock ⊢
+  aesop
+
+end FBA
 
 -- CHECK come from the "longer" file
-def quorum_of (p : Node) (Q : Set Node) : Prop := quorum Q ∧ (p ∉ W ∨ (∃ Sl ∈ slices p, Sl ⊆ Q))
+-- class PersonalQuorums {Node : Type u} (quorum_of : Node → Set Node → Prop) where
+--   quorum_assm : ∀ p p' Q, quorum_of p Q → p' ∈ Q → quorum_of p' Q
 
-lemma quorum_of_add_self (p : Node) (Q : Set Node) : quorum_of p Q → quorum (Q ∪ { p }) := by
-  intro ⟨hq, ha⟩ ; simp only [quorum, Set.mem_inter_iff, and_imp, Set.mem_insert_iff, forall_eq_or_imp] at hq ⊢
-  intro q hb hc ; simp at hb
-  cases hb with
-  | inl heq =>
-    cases ha with
-    | inl ha => subst_vars ; contradiction
-    | inr ha => subst_vars ; rcases ha with ⟨Sl, hq1, hq2⟩ ; exists Sl ; solve_by_elim [Set.subset_union_of_subset_left]
-  | inr h => specialize hq _ h hc ; rcases hq with ⟨Sl, hq1, hq2⟩ ; exists Sl ; solve_by_elim [Set.subset_union_of_subset_left]
+-- -- CHECK come from the "longer" file
+-- namespace PersonalQuorums
 
-instance : PersonalQuorums quorum_of where
-  quorum_assm := by
-    unfold quorum_of quorum ; simp
-    intro p p' Q h1 h2 h3
-    apply And.intro ; exact h1
-    by_cases p' ∈ W <;> aesop
+-- variable {Node : Type u} (quorum_of : Node → Set Node → Prop)
+-- open PersonalQuorums
 
--- CHECK come from the "longer" file
-lemma quorum_union : quorum Q → quorum Q' → quorum (Q ∪ Q') := by
-  unfold quorum ; simp
-  -- FIXME: well, `aesop` cannot handle it. why?
-  intro ha hb p hor hw ; cases hor with
-  | inl hor => specialize ha _ hor hw ; aesop (add unsafe apply Set.subset_union_of_subset_left)
-  | inr hor => specialize hb _ hor hw ; aesop (add unsafe apply Set.subset_union_of_subset_right)
+-- def quorum_of_set (S Q : Set Node) : Prop := ∃ p ∈ S, quorum_of p Q
 
--- NOTE: this definition is different from the one on the paper!
-def is_intact (I : Set Node) : Prop :=
-  I ⊆ W ∧ quorum (inst := inst) I ∧
-    (∀ Q Q', quorum (inst := project_system inst I) Q → quorum (inst := project_system inst I) Q' →
-      Q ∩ I ≠ ∅ → Q' ∩ I ≠ ∅ → Q ∩ Q' ∩ I ≠ ∅)
+-- -- NOTE: this definition is the same as the one in the DISC'19 paper,
+-- -- but different from the one in the FMBC'20 paper!
+-- -- in the FMBC'20 paper, the conclusion should be like `S ∩ Q ∩ Q' ≠ ∅`
+-- def is_intertwined (W S : Set Node) : Prop :=
+--   S ⊆ W ∧ (∀ Q Q', quorum_of_set quorum_of S Q → quorum_of_set quorum_of S Q' → W ∩ Q ∩ Q' ≠ ∅)
 
-open PersonalQuorums
-
-lemma intact_set_is_intertwined (I : Set Node) : is_intact I → is_intertwined quorum_of W I := by
-  unfold is_intact is_intertwined quorum_of_set
-  simp only [forall_exists_index, and_imp]
-  intro h1 h2 h3
-  apply And.intro ; apply h1
-  intro Q Q' x hin hq x' hin' hq'
-  have ha := quorum_of_add_self _ _ hq
-  have ha' := quorum_of_add_self _ _ hq'
-  specialize h3 _ _ (quorum_after_proj _ _ ha) (quorum_after_proj _ _ ha')
-  sorry
-
--- -- fix an intact set, and an
--- variable (I : { I : Set Node // is_intact I })
--- variable (S : { S : Set Node // is_intertwined quorum_of W S })
-
--- lemma intact_intertwined (n : Node) : n ∈ I.val → n ∈ S.val := by
---   rcases I with ⟨I, hI⟩ ; rcases S with ⟨S, hS⟩
-
--- lemma qi_intertwined (S Q1 Q2 : Set Node) (n1 n2 : Node) :
+-- -- simply by definition
+-- lemma qi_intertwined (W S Q1 Q2 : Set Node) (n1 n2 : Node) :
 --   is_intertwined quorum_of W S → n1 ∈ S → n2 ∈ S →
 --   quorum_of n1 Q1 → quorum_of n2 Q2 →
 --   ∃ n3, n3 ∈ W ∧ n3 ∈ Q1 ∧ n3 ∈ Q2 := by
+--   unfold is_intertwined quorum_of_set
+--   simp only [forall_exists_index, and_imp]
+--   intro h1 h2 h3 h4 h5 h6
+--   specialize h2 _ _ _ h3 h5 _ h4 h6
+--   rewrite [← Set.nonempty_iff_ne_empty] at h2
+--   cases h2 ; aesop
 
-end StellarQuorums
+-- end PersonalQuorums
+
+-- namespace StellarQuorums
+
+-- def project {α β : Type} (slices : β → Set (Set α)) (S : Set α) : β → Set (Set α) :=
+--   fun n => { Sl ∩ S | Sl ∈ slices n }
+
+-- -- FIXME: might be better to lift `Node` as an argument?
+-- class System where
+--   Node : Type
+--   /-- The set of well-behaved nodes. -/
+--   W : Set Node
+--   slices : Node → Set (Set Node)
+--   slices_ne : ∀ p ∈ W, slices p ≠ ∅
+
+-- def project_system (s : System) (I : Set s.Node) : System :=
+--   { Node := s.Node
+--     W := s.W
+--     slices := project s.slices I
+--     slices_ne := by
+--       unfold project
+--       have h := s.slices_ne
+--       intro p hin ; specialize h _ hin
+--       rewrite [← Set.nonempty_iff_ne_empty] at h ⊢
+--       rcases h with ⟨Sl, h⟩ ; constructor ; aesop }
+
+-- variable [inst : System]
+-- open System
+
+-- def quorum (Q : Set Node) : Prop := ∀ p ∈ Q ∩ W, ∃ Sl ∈ slices p, Sl ⊆ Q
+
+-- lemma quorum_after_proj (Q I : Set Node) : quorum (inst := inst) Q → quorum (inst := project_system inst I) Q := by
+--   rcases inst with ⟨Node, W, slices, slices_ne⟩
+--   unfold quorum project_system project ; simp
+--   intro hq p h1 h2 ; specialize hq _ h1 h2 ; rcases hq with ⟨Sl, hq1, hq2⟩
+--   exists Sl ; apply And.intro ; assumption
+--   rw [Set.subset_def] at hq2 ⊢ ; simp ; aesop     -- well, just by def
+
+-- -- CHECK come from the "longer" file
+-- def quorum_of (p : Node) (Q : Set Node) : Prop := quorum Q ∧ (p ∉ W ∨ (∃ Sl ∈ slices p, Sl ⊆ Q))
+
+-- lemma quorum_of_add (p : Node) (Q : Set Node) : p ∈ Q → p ∈ W → quorum Q → quorum_of p Q := by
+--   intro hp hw hq
+--   unfold quorum_of
+--   apply And.intro ; assumption
+--   unfold quorum at hq
+--   simp at hq ; specialize hq _ hp hw ; aesop
+
+-- def def1 (W S : Set Node) : Prop :=
+--   S ⊆ W ∧ (∀ Q Q', (∃ p ∈ S, quorum_of p Q) → (∃ p ∈ S, quorum_of p Q') → S ∩ Q ∩ Q' ≠ ∅)
+
+-- def def2 (W S : Set Node) : Prop :=
+--   S ⊆ W ∧ (∀ Q Q', quorum Q → quorum Q' → Q ∩ S ≠ ∅ → Q' ∩ S ≠ ∅ → S ∩ Q ∩ Q' ≠ ∅)
+
+-- example : ∀ S, def1 W S → def2 W S := by
+--   intro S ⟨ha, hb⟩
+--   apply And.intro ; assumption
+--   intro Q Q' hq hq' hi hi'
+--   rw [← Set.nonempty_iff_ne_empty] at hi hi'
+--   rcases hi with ⟨n, hi⟩ ; rcases hi' with ⟨n', hi'⟩
+--   simp at hi hi'
+--   rcases hi with ⟨hip, his⟩ ; rcases hi' with ⟨hip', his'⟩
+--   simp at hb
+--   have hiw : n ∈ W := by rw [Set.subset_def] at ha ; solve_by_elim
+--   have hiw' : n' ∈ W := by rw [Set.subset_def] at ha ; solve_by_elim
+--   specialize hb _ _ n his (quorum_of_add _ _ hip hiw hq) _ his' (quorum_of_add _ _ hip' hiw' hq')
+--   assumption
+
+-- example : ∀ S, def2 W S → def1 W S := by
+--   intro S ⟨ha, hb⟩
+--   apply And.intro ; assumption
+--   intro Q Q' ⟨n, hiq, ⟨hq, hqq⟩⟩ ⟨n', hiq', ⟨hq', hqq'⟩⟩
+--   have hiw : n ∈ W := by rw [Set.subset_def] at ha ; solve_by_elim
+--   have hiw' : n' ∈ W := by rw [Set.subset_def] at ha ; solve_by_elim
+--   rcases hqq with hqq | hqq ; contradiction
+--   rcases hqq' with hqq' | hqq' ; contradiction
+--   rw [← Set.nonempty_iff_ne_empty] at hi hi'
+--   rcases hi with ⟨n, hi⟩ ; rcases hi' with ⟨n', hi'⟩
+--   simp at hi hi'
+--   rcases hi with ⟨hip, his⟩ ; rcases hi' with ⟨hip', his'⟩
+--   simp at hb
+--   have hiw : n ∈ W := by rw [Set.subset_def] at ha ; solve_by_elim
+--   have hiw' : n' ∈ W := by rw [Set.subset_def] at ha ; solve_by_elim
+--   specialize hb _ _ n his (quorum_of_add _ _ hip hiw hq) _ his' (quorum_of_add _ _ hip' hiw' hq')
+--   assumption
+
+
+-- lemma quorum_of_add_self (p : Node) (Q : Set Node) : quorum_of p Q → quorum (Q ∪ { p }) := by
+--   intro ⟨hq, ha⟩ ; simp only [quorum, Set.mem_inter_iff, and_imp, Set.mem_insert_iff, forall_eq_or_imp] at hq ⊢
+--   intro q hb hc ; simp at hb
+--   cases hb with
+--   | inl heq =>
+--     cases ha with
+--     | inl ha => subst_vars ; contradiction
+--     | inr ha => subst_vars ; rcases ha with ⟨Sl, hq1, hq2⟩ ; exists Sl ; solve_by_elim [Set.subset_union_of_subset_left]
+--   | inr h => specialize hq _ h hc ; rcases hq with ⟨Sl, hq1, hq2⟩ ; exists Sl ; solve_by_elim [Set.subset_union_of_subset_left]
+
+-- instance : PersonalQuorums quorum_of where
+--   quorum_assm := by
+--     unfold quorum_of quorum ; simp
+--     intro p p' Q h1 h2 h3
+--     apply And.intro ; exact h1
+--     by_cases p' ∈ W <;> aesop
+
+-- -- CHECK come from the "longer" file
+-- lemma quorum_union : quorum Q → quorum Q' → quorum (Q ∪ Q') := by
+--   unfold quorum ; simp
+--   -- FIXME: well, `aesop` cannot handle it. why?
+--   intro ha hb p hor hw ; cases hor with
+--   | inl hor => specialize ha _ hor hw ; aesop (add unsafe apply Set.subset_union_of_subset_left)
+--   | inr hor => specialize hb _ hor hw ; aesop (add unsafe apply Set.subset_union_of_subset_right)
+
+-- -- NOTE: this definition is different from the one on the paper!
+-- def is_intact (I : Set Node) : Prop :=
+--   I ⊆ W ∧ quorum (inst := inst) I ∧
+--     (∀ Q Q', quorum (inst := project_system inst I) Q → quorum (inst := project_system inst I) Q' →
+--       Q ∩ I ≠ ∅ → Q' ∩ I ≠ ∅ → Q ∩ Q' ∩ I ≠ ∅)
+
+-- open PersonalQuorums
+
+-- lemma intact_set_is_intertwined (I : Set Node) : is_intact I → is_intertwined quorum_of W I := by
+--   unfold is_intact is_intertwined quorum_of_set
+--   simp only [forall_exists_index, and_imp]
+--   intro h1 h2 h3
+--   apply And.intro ; apply h1
+--   intro Q Q' x hin hq x' hin' hq'
+--   have ha := quorum_of_add_self _ _ hq
+--   have ha' := quorum_of_add_self _ _ hq'
+--   specialize h3 _ _ (quorum_after_proj _ _ ha) (quorum_after_proj _ _ ha')
+--   sorry
+
+-- -- -- fix an intact set, and an
+-- -- variable (I : { I : Set Node // is_intact I })
+-- -- variable (S : { S : Set Node // is_intertwined quorum_of W S })
+
+-- -- lemma intact_intertwined (n : Node) : n ∈ I.val → n ∈ S.val := by
+-- --   rcases I with ⟨I, hI⟩ ; rcases S with ⟨S, hS⟩
+
+-- -- lemma qi_intertwined (S Q1 Q2 : Set Node) (n1 n2 : Node) :
+-- --   is_intertwined quorum_of W S → n1 ∈ S → n2 ∈ S →
+-- --   quorum_of n1 Q1 → quorum_of n2 Q2 →
+-- --   ∃ n3, n3 ∈ W ∧ n3 ∈ Q1 ∧ n3 ∈ Q2 := by
+
+-- end StellarQuorums
